Nerodia/Data/PyAny.lean
@@ -1,0 +1,60 @@
+/-
+Copyright (c) 2026 Lean FRO. All rights reserved.
+Released under Apache 2.0 license as described in the file LICENSE.
+Authors: Mac Malone
+-/
+module
+public import Nerodia.Data.Py.Basic
+
+/-! # PyAny -/
+
+namespace Nerodia
+
+/--
+A special indicator signifying any acceptable value.
+This is analogous to Python's [{lit}`Any`][1].
+
+As a typing, this is propositionally equivalent to {lean}`object`,
+but it has different type class instances.
+
+[1]: https://typing.python.org/en/latest/spec/special-types.html#any
+-/
+public opaque any : Constant
+
+@[irreducible] public def Typing.any : Typing := .object
+
+public instance : CoeDep Constant any Typing := ⟨.any⟩
+
+@[simp, grind =] public theorem Typing.any_eq_object : any = object := by
+  unfold any; rfl
+
+public instance : NonemptyPy any :=
+  .intro Classical.ofNonempty (by simp)
+
+public instance : DecidablePy any := private_decl%
+  (fun _ => isTrue (by simp))
+
+/--
+A Python object of unknown type. This is analogous to Python's {lit}`Any`.
+
+As Lean is statically typed, there is little utility in using this type
+instead of {name}`PyObject` within Lean code. However, it exists to enable
+defining Python functions whose parameters or return should be left untyped.
+
+For example, a module function defined as
+
+```
+@[py_module_fn] def foo (o : PyObject) : PyObject := ...
+```
+
+will be given the type {lit}`(o: object) -> object` by Nerodia, whereas
+
+```
+@[py_module_fn] def foo (o : PyAny) : PyAny := ...
+```
+
+will have the type {lit}`(o)` with no annotated parameter or return types.
+-/
+public abbrev PyAny := PyObjectView <| Py any
+
+public instance : ViewPy any PyAny := ⟨rfl⟩
