Nerodia/Data/PyNever.lean
@@ -1,0 +1,54 @@
+/-
+Copyright (c) 2026 Lean FRO. All rights reserved.
+Released under Apache 2.0 license as described in the file LICENSE.
+Authors: Mac Malone
+-/
+module
+public import Nerodia.Data.Py.Basic
+
+/-! # PyNever -/
+
+namespace Nerodia
+
+/--
+The special form [{lit}`Never`][1], which is the {lean}`Empty` of Python.
+
+[1]: https://typing.python.org/en/latest/spec/special-types.html#never
+-/
+public opaque never : Constant
+
+/-- Python {lit}`Never`. The bottom (⊥) element of the set of typings. -/
+public def Typing.never : Typing :=
+  ofFn fun _ => False
+
+public instance : CoeDep Constant never Typing := ⟨.never⟩
+
+@[inline, irreducible, expose] -- for Nerodia compiler reduction
+public protected def TypeExpr.never : TypeExpr :=
+  ⟨"Never"⟩
+
+public instance : CoeDep Constant never TypeExpr := ⟨.never⟩
+public instance : ToTypeExpr never := ⟨never⟩
+
+@[simp, grind .] public theorem PyObject.HasType.not_never : ¬ o ⦂ never := by
+  simp [Typing.never]
+
+@[deprecated PyObject.HasType.not_never (since := "2026-09-22")]
+public abbrev Typing.not_hasType_never := @PyObject.HasType.not_never
+
+public instance : DecidablePy never := private_decl%
+  fun _ => isFalse PyObject.HasType.not_never
+
+/--
+An instance of the empty type [{lit}`Never`][1]. There are no inhabitants.
+
+[1]: https://docs.python.org/3/library/typing.html#typing.Never
+-/
+public abbrev PyNever := Py never
+
+public instance : ViewPy never PyNever := ⟨rfl⟩
+
+/-- Anything holds from an instance of the empty type (c.f., {lean}`Empty.elim`). -/
+@[macro_inline, irreducible, expose] -- for codegen
+public def PyNever.elim {α : Sort u} (self : PyNever) : α :=
+  self.toPyObject_hasType.not_never.elim
