Nerodia/Data/Typing/Ops.lean
@@ -1,0 +1,184 @@
+/-
+Copyright (c) 2026 Lean FRO. All rights reserved.
+Released under Apache 2.0 license as described in the file LICENSE.
+Authors: Mac Malone
+-/
+module
+public import Nerodia.Data.PyNever
+
+/-! # Typing Operations -/
+
+namespace Nerodia.Typing
+
+/-! ## Union -/
+
+public protected def union (T : Typing) (U : Typing) : Typing :=
+  ofFn fun o => o ⦂ T ∨ o ⦂ U
+
+public instance : Union Typing := ⟨Typing.union⟩
+
+@[grind =] public theorem union_iff_or {T U : Typing} :
+  o ⦂ T ∪ U ↔ o ⦂ T ∨ o ⦂ U
+:= by simp only [Union.union, Typing.union, ofFn_iff]
+
+@[deprecated union_iff_or (since := "2026-09-20")]
+public theorem hasType_union_iff_or {T U : Typing} :
+  o ⦂ T ∪ U ↔ o ⦂ T ∨ o ⦂ U := union_iff_or
+
+/--
+Constructs the union of two typings.
+Written as {lean}`T ∪ U`. Equivalent to the Python `T | U`.
+-/
+add_decl_doc Typing.union
+
+public instance [ToTypeExpr T] [ToTypeExpr U] : ToTypeExpr (T ∪ U) where
+  toTypeExpr:= .union (ToTypeExpr.toTypeExpr T) (ToTypeExpr.toTypeExpr U)
+
+public instance [DecidablePy T] [DecidablePy U] : DecidablePy (T ∪ U) := private_decl%
+  fun _ => decidable_of_iff' _ Typing.union_iff_or
+
+/-! ## Intersection -/
+
+public protected def inter (T : Typing) (U : Typing) : Typing :=
+  ofFn fun o => o ⦂ T ∧ o ⦂ U
+
+public instance : Inter Typing := ⟨Typing.inter⟩
+
+@[grind =] public theorem inter_iff_and {T U : Typing} :
+  o ⦂ T ∩ U ↔ o ⦂ T ∧ o ⦂ U
+:= by simp only [Inter.inter, Typing.inter, ofFn_iff]
+
+@[deprecated inter_iff_and (since := "2026-09-20")]
+public theorem hasType_inter_iff_and {T U : Typing} :
+  o ⦂ T ∩ U ↔ o ⦂ T ∧ o ⦂ U := inter_iff_and
+
+/--
+Constructs the intersection of two type predicates. Written as {lean}`T ∩ U`.
+
+Python's type system has no equivalent, but [ty][1] represents this
+as {lit}`T & U` / {lit}`Intersection[T, U]`.
+
+[1]: https://docs.astral.sh/ty/features/type-system/#intersection-types
+-/
+add_decl_doc Typing.inter
+
+public instance [DecidablePy T] [DecidablePy U] : DecidablePy (T ∩ U) := private_decl%
+  fun _ => decidable_of_iff' _ Typing.inter_iff_and
+
+/-! ## Subset (Subtype) -/
+
+public def Subset (T : Typing) (U : Typing) : Prop :=
+  ∀ o, o ⦂ T → o ⦂ U
+
+public instance : HasSubset Typing := ⟨Subset⟩
+
+/--
+{given -show}`T : Typing, U : Typing`
+{lean}`Subset T U` holds if {lean}`T` is a subtype of {lean}`U`.
+Written as {lean}`T ⊆ U`.
+-/
+add_decl_doc Subset
+
+@[grind =] public theorem subset_iff_forall {T U : Typing} :
+  T ⊆ U ↔ ∀ o, o ⦂ T → o ⦂ U
+:= Iff.intro id id
+
+public theorem Subset.hasType_of_hasType
+  {T U : Typing} (h : T ⊆ U) (ho : o ⦂ T)
+: o ⦂ U := subset_iff_forall.mp h o ho
+
+@[refl] public theorem Subset.refl (T : Typing) : T ⊆ T :=
+  subset_iff_forall.mpr fun _ => id
+
+public theorem Subset.rfl {T : Typing} : T ⊆ T :=
+  .refl T
+
+public theorem Subset.trans {T U V : Typing} (h₁ : T ⊆ U) (h₂ : U ⊆ V) : T ⊆ V :=
+  subset_iff_forall.mpr fun _ h => h₂.hasType_of_hasType (h₁.hasType_of_hasType h)
+
+end Typing
+
+public theorem PyObject.HasType.left
+  {T U : Typing} (h : o ⦂ T ∩ U) : o ⦂ T
+:= Typing.inter_iff_and.mp h |>.left
+
+public theorem PyObject.HasType.right
+  {T U : Typing} (h : o ⦂ T ∩ U) : o ⦂ U
+:= Typing.inter_iff_and.mp h |>.right
+
+public theorem PyObject.HasType.union_left
+  {T U : Typing} (h : o ⦂ T) : o ⦂ T ∪ U
+:= Typing.union_iff_or.mpr <| .inl h
+
+public instance [NonemptyPy T] : NonemptyPy (T ∪ U) :=
+  let o : Py T := Classical.ofNonempty
+  ⟨.ofPyObject o o.toPyObject_hasType.union_left⟩
+
+public theorem PyObject.HasType.union_right
+  {T U : Typing} (h : o ⦂ U) : o ⦂ T ∪ U
+:= Typing.union_iff_or.mpr <| .inr h
+
+public instance [NonemptyPy U] : NonemptyPy (T ∪ U) :=
+  let o : Py U := Classical.ofNonempty
+  ⟨.ofPyObject o o.toPyObject_hasType.union_right⟩
+
+@[deprecated PyObject.HasType.left (since := "2026-09-22")]
+public abbrev Typing.HasType.left := @PyObject.HasType.left
+
+@[deprecated PyObject.HasType.right (since := "2026-09-22")]
+public abbrev Typing.HasType.right := @PyObject.HasType.right
+
+/-! ## Inter-Operation Relations -/
+
+namespace Typing
+
+public theorem Subset.inter_left {T U : Typing} : T ∩ U ⊆ T :=
+  subset_iff_forall.mpr fun _ => .left
+
+public theorem Subset.inter_right {T U : Typing} : T ∩ U ⊆ U :=
+  subset_iff_forall.mpr fun _ => .right
+
+public theorem Subset.union_left {T U : Typing} : T ⊆ T ∪ U :=
+  subset_iff_forall.mpr fun _ => .union_left
+
+public theorem Subset.union_right {T U : Typing} : T ⊆ U ∪ T :=
+  subset_iff_forall.mpr fun _ => .union_right
+
+-- the below are `@[simp]` only because grind already handles them
+
+@[simp] public theorem Subset.object : T ⊆ object :=
+  subset_iff_forall.mpr fun _ _ => .object
+
+@[simp] public theorem union_object : T ∪ object = object := by
+  simp [Typing.ext_iff, union_iff_or]
+
+@[simp] public theorem object_union : object ∪ T = object := by
+  simp [Typing.ext_iff, union_iff_or]
+
+@[simp] public theorem inter_object : T ∩ object = T := by
+  simp [Typing.ext_iff, inter_iff_and]
+
+@[simp] public theorem object_inter : object ∩ T = T := by
+  simp [Typing.ext_iff, inter_iff_and]
+
+-- the below are `@[simp]` only because grind already handles them
+
+@[simp] public theorem Subset.never : never ⊆ T :=
+  subset_iff_forall.mpr fun _ h => h.not_never.elim
+
+@[deprecated Subset.never (since := "2026-09-11")]
+public theorem never_subset : never ⊆ T := Subset.never
+
+@[simp] public theorem union_never : T ∪ never = T := by
+  simp [Typing.ext_iff, union_iff_or]
+
+@[simp] public theorem never_union : never ∪ T = T := by
+  simp [Typing.ext_iff, union_iff_or]
+
+@[simp] public theorem inter_never : T ∩ never = never := by
+  simp [Typing.ext_iff, inter_iff_and]
+
+@[simp] public theorem never_inter : never ∩ T = never := by
+  simp [Typing.ext_iff, inter_iff_and]
+
+end Typing
