Nerodia/Data/Typing/Promotable.lean
@@ -1,0 +1,104 @@
+/-
+Copyright (c) 2026 Lean FRO. All rights reserved.
+Released under Apache 2.0 license as described in the file LICENSE.
+Authors: Mac Malone
+-/
+module
+public import Nerodia.Data.Typing.Ops
+
+/-! # Type Promotion -/
+
+namespace Nerodia
+
+/--
+Bidirectional type promotion from {lean}`U` to {lean}`T`.
+
+Promotes a concrete subtype to a concrete supertype
+(e.g., {lit}`bool` to {lit}`int`).
+-/
+public class PromotableB (T U : semiOutParam Typing) : Prop where
+  intro :: infer : U ⊆ T
+
+/--
+Type promotion from {lean}`U` to {lean}`T` chained right-to-left (i.e., downwards).
+
+Promotes a subtype to a concrete supertype (e.g., {lit}`T ∩ U` to {lit}`T`).
+-/
+public class PromotableRtl (T : semiOutParam Typing) (U : Typing) : Prop where
+  intro :: infer : U ⊆ T
+
+/--
+Type promotion from {lean}`U` to {lean}`T` chained left-to-right (i.e., upwards).
+
+Promotes a concrete subtype to a supertype (e.g., {lit}`T` to {lit}`T ∪ U`)..
+-/
+public class PromotableLtr (T : Typing) (U : semiOutParam Typing) : Prop where
+  intro :: infer : U ⊆ T
+
+/--
+Transitive chain of type promotions from {lean}`U` to {lean}`T`.
+
+Has the form: `PromotableOut* PromotableIn*`.
+-/
+public class PromotableT (T : Typing) (U : Typing) : Prop where
+  intro :: infer : U ⊆ T
+
+public instance [PromotableB T U] : PromotableRtl T U := ⟨PromotableB.infer⟩
+public instance [PromotableB T U] : PromotableLtr T U := ⟨PromotableB.infer⟩
+
+public instance [PromotableT T U] [PromotableRtl U V] : PromotableT T V :=
+  ⟨@Typing.Subset.trans V U T PromotableRtl.infer PromotableT.infer⟩
+
+public instance [PromotableLtr T U] [PromotableT U V] : PromotableT T V :=
+  ⟨@Typing.Subset.trans V U T PromotableT.infer PromotableLtr.infer⟩
+
+@[default_instance] public instance : PromotableT T T := ⟨.rfl⟩
+
+/-- Type promotion from {lean}`U` to {lean}`T`. -/
+public class Promotable (T : Typing) (U : Typing) : Prop where
+  intro :: infer : U ⊆ T
+
+public instance [PromotableT T U]  : Promotable T U := ⟨PromotableT.infer⟩
+@[default_instance] public instance : Promotable T T := ⟨.rfl⟩
+
+public theorem Subset.of_promotable [Promotable T U] : U ⊆ T :=
+  Promotable.infer
+
+public instance : Promotable T .never := ⟨.never⟩
+public instance : Promotable .object T := ⟨.object⟩
+public instance : PromotableRtl T (T ∩ U) := ⟨.inter_left⟩
+public instance : PromotableRtl U (T ∩ U) := ⟨.inter_right⟩
+public instance : PromotableLtr (T ∪ U) T := ⟨.union_left⟩
+public instance : PromotableLtr (T ∪ U) U := ⟨.union_right⟩
+
+/-! ## Promoting Objects -/
+
+public theorem PyObject.HasType.promote
+  [Promotable T U] (h : self ⦂ U) : self ⦂ T
+:= Subset.of_promotable.hasType_of_hasType h
+
+/--
+**Type promotion.**
+Casts a Python object from {lean}`U` to its supertype {lean}`T`.
+-/
+@[inline] public def Py.promote [Promotable T U] (self : Py U) : Py T :=
+  ofPyObject self self.toPyObject_hasType.promote
+
+public instance [Promotable T U] : ToPy T (Py U) := ⟨Py.promote⟩
+
+@[simp, grind =] public theorem toPy_eq_promote [Promotable T U] :
+  toPy o = Py.promote o (T := T) (U := U) := by rfl
+
+/-! ## IsSubtypeOf -/
+
+/-- Type class used to automatically infer supertypes. -/
+public class IsSubtypeOf (T U : Typing) : Prop where
+  infer_subtype : U ⊆ T
+
+export IsSubtypeOf (infer_subtype)
+
+public instance [Promotable T U] : IsSubtypeOf T U := ⟨Promotable.infer⟩
+public instance [IsSubtypeOf T U] : Promotable T U := ⟨infer_subtype⟩
+
+attribute [deprecated "Use one of the `Promotable` classes." (since := "2026-09-16")] IsSubtypeOf
+attribute [deprecated Subset.of_promotable (since := "2026-09-16")] infer_subtype
