Nerodia/Data/Typing/Raw.lean
@@ -1,0 +1,106 @@
+/-
+Copyright (c) 2026 Lean FRO. All rights reserved.
+Released under Apache 2.0 license as described in the file LICENSE.
+Authors: Mac Malone
+-/
+module
+public import Nerodia.Data.TypeExpr
+public import Nerodia.Data.Py.Raw.Type
+
+/-! # Typings -/
+
+namespace Nerodia
+
+/--
+A typing predicate for Python objects.
+
+This is the propositional equivalent of a Python type expression.
+However, it can express more complex types (e.g., intersections) than Python's
+base type system and is thus closer in power to the type system of Python's
+more advanced type checkers (e.g., [{lit}`ty`][1]).
+
+[1]: https://github.com/astral-sh/ty
+-/
+@[irreducible, expose] -- for codegen
+public def Typing : Type :=
+  Internal.Py.Raw → Prop
+
+/--
+Associates a Python type expression with a Nerodia type predicate.
+
+This class is used by the Nerodia compiler to generate Python type annotations.
+For this to work, all instances must be publicly reducible to {lean}`String`.
+Thus, definitions they use must be marked {attr}`@[expose]`.
+-/
+public class ToTypeExpr (T : Typing) where
+  toTypeExpr : TypeExpr
+
+namespace Typing
+export ToTypeExpr (toTypeExpr)
+end Typing
+
+/--
+Auxiliary type used for values representing a static Python constant.
+
+Similar to {lean}`Lean.Parser.Category`, definitions of this type have no
+content, they simply reserve names that can be coerced into other types (e.g.,
+{lean}`TypeExpr` or {lean}`Typing`) via {lean}`CoeDep`.
+
+**Users of Nerodia should not define values of this type themselves.**
+-/
+public structure Constant where
+  private mk ::
+    private val : NonScalar
+    deriving Inhabited
+
+unseal Typing in
+public def Internal.Py.Raw.HasType (T : Typing) (o : Py.Raw) : Prop :=
+  T o
+
+unseal Typing in
+public theorem Internal.Py.Raw.HasType.ext
+  {T U : Typing} (h : ∀ o, HasType T o ↔ HasType U o) : T = U
+:= funext fun o => propext (h o)
+
+@[deprecated "Use `PyObject.HasType` or `o ⦂ T` instead."  (since := "2026-09-19")]
+public protected abbrev Typing.HasType (T : Typing) (o : Internal.Py.Raw) : Prop :=
+  o.HasType T
+
+export Typing (HasType)
+
+unseal Typing in
+public def Internal.Nerodia.Typing.ofRawFn (p : Py.Raw → Prop) : Typing :=
+  p
+
+unseal Typing in
+open Internal in
+public theorem Internal.Py.Raw.HasType.ofRawFn_iff :
+  HasType (.ofRawFn p) o ↔ p o
+:= Iff.intro id id
+
+/-! ## object -/
+
+/--
+The ultimate Python base class, [{lit}`object`][1].
+
+[1]: https://docs.python.org/3/library/functions.html#object
+-/
+public opaque object : Constant
+
+open Internal in
+/-- Python {lit}`object`. The top (⊤) element of the set of typings. -/
+public def Typing.object : Typing :=
+  .ofRawFn fun _ => True
+
+public instance : CoeDep Constant object Typing := ⟨.object⟩
+
+@[inline, irreducible, expose] -- for Nerodia compiler reduction
+public protected def TypeExpr.object : TypeExpr :=
+  ⟨"object"⟩
+
+public instance : CoeDep Constant object TypeExpr := ⟨.object⟩
+public instance : ToTypeExpr object := ⟨object⟩
+
+open Internal Nerodia in
+public theorem Internal.Py.Raw.HasType.object : HasType .object o := by
+  simp [Typing.object, Typing.ofRawFn, HasType]
